Cleanup Partition.dfy

Partition.dfy
@@ -1,193 +1,19 @@
+include "Utils.dfy"
+include "EquivClass.dfy"
 include "Tree.dfy"
-
-class EquivClass {
-  ghost var repr: set<EquivClass>;
-  // var height: nat;
-  var parent: EquivClass?;
-
-  predicate Valid()
-    reads this, repr
-  {
-    if parent == null then
-      repr == {this}
-      // && height == 0
-    else
-      parent in repr
-      && this !in parent.repr
-      // && height == 1 + parent.height  // MAL
-      && repr == {this} + parent.repr
-      // && repr >= {this} + parent.repr
-      && parent.Valid()
-  }
-
-  constructor()
-    ensures Valid()
-    ensures parent == null
-    ensures fresh(repr)
-  {
-    // height := 0;
-    parent := null;
-    repr := {this};
-  }
-
-  predicate IsChildOf(p: EquivClass)
-    reads this, repr
-    // requires Valid()
-  {
-    parent == p
-  }
-
-  // The reflexive-transitive closure of `IsChildOf` (on valid EquivClasses)
-  predicate IsDescOf(p: EquivClass)
-    reads this, repr
-    // requires Valid()
-  {
-    p in repr
-  }
-
-  static lemma IsDescOfRefl(a: EquivClass)
-    requires a.Valid()
-    ensures a.IsDescOf(a)
-  {}
-
-  // static lemma IsDescOfWeakenRight(a: EquivClass, b: EquivClass)
-  //   requires a.Valid() && b.Valid()
-  //   requires b.parent != null
-  //   requires a.IsDescOf(b)
-  //   ensures a.IsDescOf(b.parent)
-
-  // static lemma IsDescOfWeakenLeft(a: EquivClass, b: EquivClass)
-  //   requires a.Valid() && b.Valid()
-  //   requires a.parent != null
-  //   requires a.IsDescOf(b)
-  //   ensures a.parent.IsDescOf(b)
-
-  // static lemma IsDescOfWeakenLeftPrime(a: EquivClass, b: EquivClass)
-  //   requires a.Valid() && b.Valid()
-  //   requires a.parent != null
-  //   requires !a.parent.IsDescOf(b)
-  //   ensures !a.IsDescOf(b)
-  // {
-  //   if a.IsDescOf(b) {
-  //     IsDescOfWeakenLeft(a, b);
-  //   }
-  // }
-
-  static lemma IsDescOfTrans(a: EquivClass, b: EquivClass, c: EquivClass)
-    decreases a.repr
-    requires a.Valid()
-    requires a.IsDescOf(b) && b.IsDescOf(c)
-    ensures a.IsDescOf(c)
-  {
-    if a.parent != null && a != b {
-      IsDescOfTrans(a.parent, b, c);
-    }
-  }
-
-  // static lemma IsDescOfAntisym(a: EquivClass, b: EquivClass)
-  //   decreases b.repr
-  //   requires a.Valid() && b.Valid()
-  //   requires a != b
-  //   requires a.IsDescOf(b)
-  //   ensures !b.IsDescOf(a)
-  // {
-  //   if b.parent != a && b.parent != null {
-  //     IsDescOfWeakenRight(a, b);
-  //     IsDescOfAntisym(a, b.parent);
-  //   }
-  // }
-
-  // static lemma IsDescOfTransPrime(a: EquivClass, b: EquivClass, c: EquivClass)
-  //   decreases a.repr
-  //   requires a.Valid() && b.Valid() && c.Valid()
-  //   requires !a.IsDescOf(b) && b.IsDescOf(c)
-  //   ensures !a.IsDescOf(c)
-  // {
-  //   if a.parent != null && a != b {
-  //     if a != c {
-  //       IsDescOfTransPrime(a.parent, b, c);
-  //     } else {
-  //       assert !a.IsDescOf(b);
-  //       assert b.IsDescOf(a);
-  //       IsDescOfAntisym(b, a);
-  //       // assert a.IsDescOf(b);
-  //       assert !a.IsDescOf(a);
-  //       assert !a.IsDescOf(c);
-  //     }
-  //   }
-  // }
-}
-
-function method BigUnion<A>(S: set<set<A>>): set<A>
-{
-  set X, x | X in S && x in X :: x
-}
-
-function method elems<A>(l: array<A>): set<A>
-  reads l
-{
-  set x | x in l[..]
-}
-
-// class Tree {
-//   var root: EquivClass;
-//   var children: set<Tree>;
-
-//   constructor Node(r: EquivClass, cs: set<Tree>)
-//   {
-//     root := r;
-//     children := cs;
-//   }
-
-//   function method Elems(): set<EquivClass>
-//     reads this
-//   {
-//     {root} + set y, c | c in children && y in c.Elems() :: y
-//   }
-
-//   predicate Valid()
-//     decreases this
-//     // reads elemsTree(t)
-//     // reads set c | c in children :: c.root
-//     // reads set c | c in children :: c.root.parent
-//   {
-//     forall c | c in children ::
-//       c.root.parent == root
-//       // && c.root.height == p.height + 1
-//       && c.Valid()
-//   }
-// }
 
 predicate ValidTree(t: Tree<EquivClass>)
   decreases t
   reads set c | c in elemsTree(t) :: c`parent
 {
-  forall c | c in t.children ::
+  (forall c | c in t.children ::
     assert elemsTree(c) <= elemsTree(t);
     c.root.parent == t.root
     && t.root !in elemsTree(c)
-    && ValidTree(c)
-}
-
-predicate ValidTreeRepr(t: Tree<EquivClass>)
-  decreases t
-{
-  (forall c | c in t.children ::
-    ValidTreeRepr(c))
+    && ValidTree(c))
   && (forall r, s | r != s && r in t.children && s in t.children ::
-    elemsTree(r) !! elemsTree(s))
+      elemsTree(r) !! elemsTree(s))
 }
-
-// predicate ValidTreeRepr(t: Tree<EquivClass>)
-//   decreases t
-//   reads t.root, t.root.repr
-//   requires t.root.Valid()
-// {
-//   (forall c | c != t.root && c in elemsTree(t) ::
-//     c !in t.root.repr)
-//   && (forall r, s | r != s && r in t.children && s in t.children ::
-//     elemsTree(r) !! elemsTree(s))
-// }
 
 class Partition {
   var classes: array<EquivClass>;
@@ -210,45 +36,36 @@ class Partition {
     && (forall j, k | 0 <= j < k < classes.Length :: classes[j] != classes[k])
   }
 
-  // constructor(size: nat)
-  //   ensures Valid()
-  // {
-  //   new;  // ¿¿¿¿qué hace esto???? .-.
-  //   var i := 0;
-  //   var temp := new EquivClass?[size](_ => null);
-  //   while i < size
-  //     modifies temp
-  //     invariant 0 <= i <= size
-  //     invariant forall j | 0 <= j < i :: temp[j] != null
-  //     invariant forall j, k | 0 <= j < k < i :: temp[j] != temp[k]
-  //     invariant forall j | 0 <= j < i :: temp[j].parent == null && temp[j].Valid()
-  //   {
-  //     temp[i] := new EquivClass();
-  //     i := i + 1;
-  //   }
-  //   classes := new EquivClass[size](
-  //     i requires 0 <= i < size reads temp => temp[i]
-  //   );
-  // }
-
-  // lemma ReprSubSet(e: EquivClass)
-  //   requires e in classes[..]
-  //   requires Valid()
-  //   ensures multiset(e.repr) <= multiset(classes[..])
+  constructor(size: nat)
+    ensures Valid()
+  {
+    new;
+    var i := 0;
+    var temp := new EquivClass?[size](_ => null);
+    while i < size
+      modifies temp
+      invariant 0 <= i <= size
+      invariant forall j | 0 <= j < i :: temp[j] != null
+      invariant forall j, k | 0 <= j < k < i :: temp[j] != temp[k]
+      invariant forall j | 0 <= j < i :: temp[j].parent == null && temp[j].Valid()
+    {
+      temp[i] := new EquivClass();
+      i := i + 1;
+    }
+    classes := new EquivClass[size](
+      i requires 0 <= i < size reads temp => temp[i]
+    );
+  }
 
   function Descendants(p: EquivClass): set<EquivClass>
     reads this, classes, elems(classes), ValidReads()
-    // requires Valid()
     requires p in classes[..]
-    // ensures Descendants(p)
-    //   == (set c: EquivClass | c in classes[..] && c.IsChildOf(p) :: c)
   {
     set c | c in classes[..] && c.IsDescOf(p)
   }
 
   function Children(p: EquivClass): set<EquivClass>
     reads this, classes, elems(classes), ValidReads()
-    // requires Valid()
     requires p in classes[..]
   {
     set c | c in classes[..] && c.IsChildOf(p)
@@ -370,7 +187,7 @@ class Partition {
     }
   }
 
-  lemma ForallDisjointDescendants(p: EquivClass)
+  lemma AllDisjointDescendants(p: EquivClass)
     requires Valid()
     requires p in classes[..]
     ensures forall c, d
@@ -392,16 +209,9 @@ class Partition {
     requires p in classes[..]
     ensures elemsTree(DescendantsTree(p)) == Descendants(p)
     ensures ValidTree(DescendantsTree(p))
-    // ensures forall c | c != p && c in elemsTree(DescendantsTree(p)) :: c !in p.repr
-    ensures ValidTreeRepr(DescendantsTree(p))
-    // ensures forall c, d
-    //   | c in elemsTree(DescendantsTree(p))
-    //   && d in elemsTree(DescendantsTree(p))
-    //   && c.IsDescOf(d)
-    //   :: c !in d.repr
   {
     ChildrenDescendants(p);
-    ForallDisjointDescendants(p);
+    AllDisjointDescendants(p);
     Node(
       p,
       set c: EquivClass | c in classes[..] && c.IsChildOf(p) ::
@@ -414,11 +224,9 @@ class Partition {
     requires forall c | c in elemsTree(dt) :: c in classes[..]
     requires dt.root.Valid()
     requires ValidTree(dt)
-    requires ValidTreeRepr(dt)
     requires forall c | c != dt.root && c in elemsTree(dt) :: c !in dt.root.repr
     ensures forall c | c in elemsTree(dt) :: c.Valid()
     ensures ValidTree(dt)
-    ensures ValidTreeRepr(dt)
     ensures forall c | c in elemsTree(dt) :: c.repr <= elemsTree(dt) + dt.root.repr
   {
     var p := dt.root;
@@ -429,7 +237,6 @@ class Partition {
       invariant children <= cs
       invariant dt.root.Valid()
       invariant ValidTree(dt)
-      invariant ValidTreeRepr(dt)
       invariant forall c, d: EquivClass | c in children && d in elemsTree(c) :: d.Valid()
       invariant forall c, d | c != d && c in children && d in children ::
         elemsTree(c) !! elemsTree(d)
@@ -437,19 +244,9 @@ class Partition {
         d.repr <= elemsTree(c) + dt.root.repr
     {
       var ct: Tree<EquivClass>; ct :| ct in cs - children;
-      assert forall c, d: EquivClass | c in children && d in elemsTree(c) :: d.Valid();
-      assert ct.root !in dt.root.repr;
-      assert forall c | c in children :: elemsTree(c) !! elemsTree(ct);
-      assert forall c, d: EquivClass | c in children && d in elemsTree(c) :: ct.root !in d.repr;
       ct.root.repr := {ct.root} + p.repr;
-      assert forall c, d: EquivClass | c in children && d in elemsTree(c) :: d.Valid();
-      assert forall c, d: EquivClass, e: EquivClass
-        | c in children && d in elemsTree(c) && e in elemsTree(ct) && e != ct.root
-        :: e !in d.repr;
       RepairDescendants(ct);
-      assert forall c, d: EquivClass | c in children && d in elemsTree(c) :: d.Valid();
       children := children + {ct};
-      assert forall c, d: EquivClass | c in children && d in elemsTree(c) :: d.Valid();
     }
     assert cs - children == {};
     assert children <= cs;
@@ -457,105 +254,9 @@ class Partition {
     assert cs == children;
   }
 
-  // ghost method RepairDescendants(p: EquivClass, dt: Tree<EquivClass>)
-  //   modifies p, elemsTree(dt)
-  //   requires p in classes[..]
-  //   requires p.Valid()
-  //   requires elemsTree(dt) == Descendants(p)
-  //   ensures forall c | c in elemsTree(dt) :: c.Valid()
-  // {
-  //   match dt {
-  //     case Node(p_, cs) => {
-  //       // assert p_ == p;
-  //       var children := {};
-  //       while cs - children != {}
-  //         decreases cs - children
-  //         modifies BigUnion(set c | c in cs :: elemsTree(c))
-  //         invariant forall c | c in children ::
-  //           c.root.Valid() && forall d | d in elemsTree(dt) :: d.Valid()
-  //       {
-  //         var c;
-  //         c :| c in (cs - children);
-  //         c.root.repr := {c.root} + p.repr;
-  //         RepairDescendants(c.root, c);
-  //         children := children + {c};
-  //       }
-  //     }
-  //   }
-  // }
-
-  // ghost method RepairChild(p: EquivClass, dt: Tree<EquivClass>)
-  //   modifies elemsTree(dt)
-  //   requires dt.root.IsChildOf(p)
-  //   ensures ValidTree(dt)
-
-  // ghost method RepairDescendants(dt: Tree<EquivClass>)
-  //   modifies dt.root, elemsTree(dt)
-  //   requires forall c | c in elemsTree(dt) :: c in classes[..]
-  //   requires dt.root.Valid()
-  //   requires ValidTree(dt)
-  //   requires ValidTreeRepr(dt)
-  //   ensures forall c | c in elemsTree(dt) :: c.Valid()
-  //   ensures ValidTree(dt)
-  //   ensures ValidTreeRepr(dt)
-  // {
-  //   match dt {
-  //     case Node(p, cs) => {
-  //       var children := {};
-  //       while cs - children != {}
-  //         decreases cs - children
-  //         invariant children <= cs
-  //         invariant Node(p, cs) == dt
-  //         invariant p.Valid()
-  //         invariant ValidTree(dt)
-  //         invariant ValidTreeRepr(dt)
-  //         invariant forall c, d | c in children && d in elemsTree(c) :: d.Valid()
-  //         invariant forall ct, c, dt
-  //           | ct in children && c in elemsTree(ct) && dt in cs - children
-  //           :: dt.root !in c.repr
-  //       {
-  //         assert forall c, d | c in children && d in elemsTree(c) :: d.Valid();
-  //         var ct; ct :| ct in cs - children;
-  //         assert ct.root in elemsTree(ct);
-  //         assert ct.root.IsChildOf(p);
-  //         assert forall c, d | c in children && d in elemsTree(c) :: d.Valid();
-  //         assert ct in cs - children;
-  //         assert ct !in children;
-  //         assert forall c, d | c in children && d in elemsTree(c) :: d.Valid();
-  //         ct.root.repr := {ct.root} + p.repr;
-  //         assert forall c, d | c in children && d in elemsTree(c) :: d.Valid();
-  //         assert elemsTree(ct) <= elemsTree(dt);
-  //         assert ct.root.parent == p;
-  //         assert p.Valid();
-  //         assert ct.root.parent.Valid();
-  //         assert ct.root.Valid();
-  //         assert elemsTree(ct) !! BigUnion(set t | t in children :: elemsTree(t));
-  //         assert forall c, d, e | c in children && d in elemsTree(c) && e in d.repr :: e !in elemsTree(ct);
-  //         RepairDescendants(ct);
-  //         assert elemsTree(ct) <= elemsTree(dt);
-  //         assert ct.root.Valid();
-  //         assert forall c, d | c in children && d in elemsTree(c) :: d.Valid();
-  //         assert forall d | d in elemsTree(ct) :: d.Valid();
-  //         children := children + {ct};
-  //       }
-  //       assert cs - children == {};
-  //       assert children <= cs;
-  //       assert cs - children + children == {} + children;
-  //       assert cs == children;
-  //     }
-  //   }
-  // }
-
-  // ghost method repair(e: EquivClass, c: EquivClass, top: EquivClass)
-  //   modifies e
-  // {
-  //   e.repr := e.repr - c.repr;
-  //   e.repr := e.repr + {c, top};
-  // }
-
-  method findAux(c: EquivClass) returns (res: EquivClass)
+  method FindAux(c: EquivClass) returns (res: EquivClass)
     decreases c.repr
-    modifies multiset(classes[..])
+    modifies elems(classes)
     requires c in classes[..]
     requires Valid()
     requires c.Valid()
@@ -570,7 +271,7 @@ class Partition {
     if c.parent == null {
       return c;
     } else {
-      res := findAux(c.parent);
+      res := FindAux(c.parent);
       ghost var dt := DescendantsTree(c);
       c.parent := res;
       // c.height := 1;
@@ -590,16 +291,14 @@ class Partition {
     }
   }
 
-  method find(i: nat) returns (res: EquivClass)
-    modifies this, classes
-    modifies set x | x in classes[..]
-    modifies BigUnion(set e: EquivClass | e in classes[..] :: e.repr)
+  method Find(i: nat) returns (res: EquivClass)
+    modifies elems(classes)
     requires Valid()
     requires 0 <= i < classes.Length
     ensures res.parent == null
     ensures res.Valid()
     ensures Valid()
   {
-    res := findAux(classes[i]);
+    res := FindAux(classes[i]);
   }
 }
