EquivClass.dfy
@@ -1,0 +1,99 @@
+class EquivClass {
+  ghost var repr: set<EquivClass>;
+  // var height: nat;
+  var parent: EquivClass?;
+
+  predicate Valid()
+    reads this, repr
+  {
+    if parent == null then
+      repr == {this}
+      // && height == 0
+    else
+      parent in repr
+      && this !in parent.repr
+      // && height == 1 + parent.height  // MAL
+      && repr == {this} + parent.repr
+      // && repr >= {this} + parent.repr
+      && parent.Valid()
+  }
+
+  constructor()
+    ensures Valid()
+    ensures parent == null
+    ensures fresh(repr)
+  {
+    // height := 0;
+    parent := null;
+    repr := {this};
+  }
+
+  predicate IsChildOf(p: EquivClass)
+    reads this, repr
+    // requires Valid()
+  {
+    parent == p
+  }
+
+  // The reflexive-transitive closure of `IsChildOf` (on valid EquivClasses)
+  predicate IsDescOf(p: EquivClass)
+    reads this, repr
+    // requires Valid()
+  {
+    p in repr
+  }
+
+  static lemma IsDescOfRefl(a: EquivClass)
+    requires a.Valid()
+    ensures a.IsDescOf(a)
+  {}
+
+  static lemma IsDescOfWeakenRight(a: EquivClass, b: EquivClass)
+    decreases a.repr
+    requires a.Valid() && b.Valid()
+    requires b.parent != null
+    requires a.IsDescOf(b)
+    ensures a.IsDescOf(b.parent)
+  {
+    if a != b && a.parent != null {
+      IsDescOfWeakenRight(a.parent, b);
+    }
+  }
+
+  static lemma IsDescOfWeakenLeft(a: EquivClass, b: EquivClass)
+    decreases a.repr
+    requires a.Valid() && b.Valid()
+    requires a.parent != null
+    requires a != b
+    requires a.IsDescOf(b)
+    ensures a.parent.IsDescOf(b)
+  {
+    if a.parent != b && b.parent != null{
+      IsDescOfWeakenLeft(a.parent, b);
+    }
+  }
+
+  static lemma IsDescOfTrans(a: EquivClass, b: EquivClass, c: EquivClass)
+    decreases a.repr
+    requires a.Valid()
+    requires a.IsDescOf(b) && b.IsDescOf(c)
+    ensures a.IsDescOf(c)
+  {
+    if a.parent != null && a != b {
+      IsDescOfTrans(a.parent, b, c);
+    }
+  }
+
+  static lemma IsDescOfAntisym(a: EquivClass, b: EquivClass)
+    decreases b.repr
+    requires a.Valid() && b.Valid()
+    requires a != b
+    requires a.IsDescOf(b)
+    ensures !b.IsDescOf(a)
+  {
+    if b.parent != a && b.parent != null {
+      IsDescOfWeakenRight(a, b);
+      IsDescOfAntisym(a, b.parent);
+    }
+  }
+}
