Utils.dfy
@@ -1,0 +1,10 @@
+function method BigUnion<A>(S: set<set<A>>): set<A>
+{
+  set X, x | X in S && x in X :: x
+}
+
+function method elems<A>(l: array<A>): set<A>
+  reads l
+{
+  set x | x in l[..]
+}
